investigations/bedrock2/RiscvMachineWithCavaDevice/Bedrock2ToCava.v
@@ -3,6 +3,7 @@ Require Import Coq.Lists.List. Import ListNotations.
 Require Import coqutil.Word.Interface coqutil.Map.Interface.
 Require Import coqutil.Map.OfListWord.
 Require Import coqutil.Datatypes.PropSet.
+Require Import coqutil.Tactics.Simp.
 Require Import riscv.Platform.MetricRiscvMachine.
 Require Import riscv.Utility.FreeMonad.
 Require Import riscv.Utility.runsToNonDet.
@@ -26,6 +27,7 @@ Section WithParams.
           {state_machine_params: StateMachineSemantics.parameters.parameters 32 word mem}
           {state_machine_params_ok: StateMachineSemantics.parameters.ok state_machine_params}
           {D: device}
+          (device_state_related: StateMachineSemantics.parameters.state -> D -> Prop)
           (sched: schedule).
 
   Open Scope ilist_scope.
@@ -34,18 +36,18 @@ Section WithParams.
     MMIO.word := word;
     MMIO.word_ok := _;
     MMIO.word_riscv_ok := _;
-    MMIO.mem := SortedListWord.map _ _;
-    MMIO.mem_ok := _;
-    MMIO.locals := _;
-    MMIO.locals_ok := _;
+    MMIO.mem := mem;
+    MMIO.mem_ok := mem_ok;
+    MMIO.locals := Registers;
+    MMIO.locals_ok := Registers_ok;
     MMIO.funname_env := SortedListString.map;
     MMIO.funname_env_ok := SortedListString.ok;
   |}.
 
   Global Instance pipeline_params: Pipeline.parameters := {|
     Pipeline.W := _;
-    Pipeline.mem := _;
-    Pipeline.Registers := _;
+    Pipeline.mem := mem;
+    Pipeline.Registers := Registers;
     Pipeline.string_keyed_map := _;
     Pipeline.ext_spec := StateMachineSemantics.ext_spec;
     Pipeline.compile_ext_call :=
@@ -55,6 +57,20 @@ Section WithParams.
     Pipeline.RVM := MetricMinimalMMIO.IsRiscvMachine;
     Pipeline.PRParams := _
   |}.
+
+  Global Instance Pipeline_assumptions : Pipeline.assumptions.
+  Proof.
+    constructor.
+    { apply MMIO.word_riscv_ok. }
+    { exact MMIO.funname_env_ok. }
+    { exact MMIO.locals_ok. }
+    { unfold Pipeline.PRParams, pipeline_params.
+      eapply MetricMinimalMMIO.MetricMinimalMMIOSatisfiesPrimitives. }
+    { exact (@FlatToRiscv_hyps MMIO_compiler_params state_machine_params). }
+    { exact (ext_spec_ok (p := @state_machine_params)). }
+    { exact (compile_ext_call_correct (state_machine_parameters_ok:=state_machine_params_ok)). }
+    { reflexivity. }
+  Qed.
 
   Definition regs_initialized(regs: Registers): Prop :=
     forall r : Z, 0 < r < 32 -> exists v : word, map.get regs r = Some v.
@@ -79,33 +95,66 @@ Section WithParams.
       mach.(getPc) = pc /\
       mach.(getNextPc) = word.add mach.(getPc) (word.of_Z 4) /\
       regs_initialized mach.(getRegs) /\
-      map.get mach.(getRegs) RegisterNames.sp = Some stack_pastend (*/\
-      TODO we should have some conditions that imply these, but don't use the notion of
-      MMIO, because MMIO is only used at the intermediate spec that we want to cancel out
-      map.undef_on m StateMachineSemantics.parameters.isMMIOAddr /\
-      disjoint (of_list xAddrs) StateMachineSemantics.parameters.isMMIOAddr *) .
+      map.get mach.(getRegs) RegisterNames.sp = Some stack_pastend /\
+      (* Note: the concept of isMMIOAddr appears in the bedrock2 program specs, so it's
+         fine if it also appears in the combined theorem *)
+      map.undef_on mach.(getMem) StateMachineSemantics.parameters.isMMIOAddr /\
+      disjoint (of_list mach.(getXAddrs)) StateMachineSemantics.parameters.isMMIOAddr.
 
   Lemma bedrock2_and_cava_system_correct: forall functions instrs pos_map required_stack_space
         f_entry_name fbody mc p_functions f_entry_rel_pos stack_start stack_pastend
-      finstrs p_call mH Rdata Rexec (initialL: ExtraRiscvMachine D) steps_done postH,
+        p_call mH Rdata Rexec (initialL: ExtraRiscvMachine D) steps_done postH,
       ExprImp.valid_funs functions ->
       compile functions = Some (instrs, pos_map, required_stack_space) ->
       map.get functions f_entry_name = Some ([], [], fbody) ->
       map.get pos_map f_entry_name = Some f_entry_rel_pos ->
       required_stack_space <= word.unsigned (word.sub stack_pastend stack_start) / bytes_per_word ->
+      word.unsigned (word.sub stack_pastend stack_start) mod bytes_per_word = 0 ->
+      (exists s, StateMachineSemantics.parameters.is_initial_state s /\
+                 device_state_related s initialL.(getExtraState)) ->
       Semantics.exec.exec functions fbody initialL.(getLog) mH map.empty mc
-           (fun t' m' l' mc' => postH m') ->
-      machine_ok p_functions f_entry_rel_pos stack_start stack_pastend finstrs p_call
+           (fun t' m' l' mc' => postH m' /\ exists s' tnew, t' = tnew ++ initialL.(getLog)
+                                                            /\ execution tnew s') ->
+      machine_ok p_functions f_entry_rel_pos stack_start stack_pastend instrs p_call
                  p_call mH Rdata Rexec initialL ->
       exists steps_remaining finalL mH',
         run_rec sched steps_done steps_remaining initialL = (Some tt, finalL) /\
-        machine_ok p_functions f_entry_rel_pos stack_start stack_pastend finstrs p_call
+        machine_ok p_functions f_entry_rel_pos stack_start stack_pastend instrs p_call
                    (word.add p_call (word.of_Z 4)) mH' Rdata Rexec finalL /\
-        postH mH'.
+        postH mH' /\
+        finalL.(getLog) = initialL.(getLog) (* no external interactions happened *).
   Proof.
     intros.
-    pose proof @Pipeline.compiler_correct as P.
-    pose proof stateMachine_to_cava as Q.
-  Admitted.
+    destruct initialL as (mach & d). destruct mach as [r pc npc m xAddrs t].
+    unfold machine_ok in *; cbn -[map.get map.empty] in *. simp.
+    edestruct (stateMachine_to_cava device_state_related)
+      as (steps_remaining & finalL & finalH & Rn & Rfinal & Pf).
+    2: {
+      pose proof Pipeline.compiler_correct as P.
+      unfold FlatToRiscvCommon.runsTo, GoFlatToRiscv.mcomp_sat,
+        mcomp_sat, FlatToRiscvCommon.PRParams in P.
+      cbn -[map.get map.empty] in P.
+      eapply P with (initial := {| MetricRiscvMachine.getMachine := {| getPc := _ |} |});
+        clear P; cbn -[map.get map.empty]; try eassumption.
+      1: exact H6.
+      unfold LowerPipeline.machine_ok; cbn -[map.get map.empty];
+        ssplit; try eassumption; try reflexivity.
+    }
+    2: {
+      inversion Rfinal. subst; clear Rfinal.
+      unfold LowerPipeline.machine_ok in *. cbn -[map.get map.empty] in *.
+      simp.
+      eexists _, {| getMachine := {| getLog := t |} |}, _; cbn -[map.get map.empty]. ssplit.
+      1: exact Rn.
+      all: cbn -[map.get map.empty].
+      all: try eassumption.
+      all: try reflexivity.
+    }
+    (* `related` holds at beginning: *)
+    change t with ([] ++ t) at 2.
+    econstructor. 1: unfold execution. all: try eassumption.
+    Unshelve.
+    all: do 2 constructor.
+  Qed.
 
 End WithParams.
